simplifying assumptions

case_studies/HamiltonBlum/Blum_Basics.ec
@@ -5,16 +5,16 @@ require  GenericSigmaProtocol.
 require CommitmentSpecial.
 clone include CommitmentSpecial with type message <- bool.
 
-
-type graph = bool list.         (* n * n list representin n x n matrix *)
-
 op K : int.
 axiom K_pos : 0 < K.
+
+type graph = bool list.         (* K * K list representing K x K matrix *)
 
 type hc_prob = graph.
 type hc_wit  = int list.
 type hc_com  = commitment list.
-type hc_resp = (permutation * (opening list) , hc_wit * (opening list)) sum.
+type hc_resp = (permutation * (opening list), 
+                 hc_wit * (opening list)) sum.
 
 op compl_graph     : int -> graph.
 op compl_graph_cyc : int -> int list = range 0.
@@ -22,41 +22,32 @@ op compl_graph_cyc : int -> int list = range 0.
 op permute_graph (p : permutation) (g : graph) : graph.
 op permute_witness : permutation -> hc_wit -> hc_wit = map.
 
-(* projects the witness up-fron
-   prj (1,2,3) [x11 x12 x13 x21 x22 x23 x31 x32 x33]
-
-    project out the positions of the cycle (1,2)(2,3)(3,1)
-           [x12 x23 x31] ++ [x11 x13 x21 x22 x32 x33]
-*)
 op prj_path ['a]  : hc_wit -> 'a list -> 'a list.
-
 
 op hc_verify (p : hc_prob) (c : hc_com) (b : bool)  (r : hc_resp) : bool =
  with r = (Left x) => b /\ all Ver (zip (permute_graph x.`1 p) (zip c x.`2))
-                         /\ size c = K * K
-                         /\ size p = K * K
-                         /\ size x.`2 = K * K
-
- with r = (Right x) => ! b /\ uniq x.`1
-                        /\ size x.`1 = K
                         /\ size c = K * K
-                        /\ size x.`2 = K
-                        /\ all Ver 
-                             (zip (nseq K true) 
-                                    (zip ((prj_path x.`1 c)) x.`2))
-                        /\ perm_eq x.`1 (range 0 K)
-                        /\ size p = K * K.
+                        /\ size p = K * K
+                        /\ size x.`2 = K * K
+ with r = (Right x) => ! b /\ uniq x.`1
+                           /\ size x.`1 = K
+                           /\ size c = K * K
+                           /\ size x.`2 = K
+                           /\ all Ver 
+                                 (zip (nseq K true) 
+                                   (zip ((prj_path x.`1 c)) x.`2))
+                           /\ perm_eq x.`1 (range 0 K)
+                           /\ size p = K * K.
 
-
-op IsHC (x : hc_prob * hc_wit) : bool 
-  = 
-    let g = x.`1 in
-    let w = x.`2 in
+op completeness_relation (g : hc_prob) (w : hc_wit) : bool  = 
      K = size w /\ 
      K * K = size g /\ 
      perm_eq w (range 0 K) /\ 
      nseq K true = prj_path w g.
 
+op soundness_relation = completeness_relation.
+
+op zk_relation = completeness_relation.
 
 clone export GenericSigmaProtocol as BlumProtocol with 
   type statement       <- hc_prob,
@@ -66,41 +57,55 @@ clone export GenericSigmaProtocol as BlumProtocol with
   type challenge       <- bool,
   op challenge_set     <=  (false :: true :: []),
   op verify_transcript <= fun p (x : transcript) => hc_verify p x.`1 x.`2 x.`3,
-  op soundness_relation    <= fun x y => IsHC (x, y),
-  op completeness_relation <= fun x y => IsHC (x, y),
-  op zk_relation           <= fun x y => IsHC (x, y).
+  op soundness_relation    <- soundness_relation,
+  op completeness_relation <- completeness_relation,
+  op zk_relation           <- zk_relation.
  
 
-(* require Djoinmap. *)
-(* clone import Djoinmap as DJMM with type a <- bool,  *)
-(*                                    type b <- commitment * opening, *)
-(*                                    op   d <- Com. *)
+module HonestProver : HonestProver  = {
+  var g : graph                 (* n*n adj. matrix *)
+  var prm : permutation         
+  var w : hc_wit                
+  var fal : bool list           
+  var pi_gwco : (commitment * opening) list
+  var pi_w : hc_wit
+  
+  proc commitment(p_a : hc_prob, w_a : hc_wit)  = {
+    g <- p_a;
+    w     <- w_a;
+    prm   <$ perm_d K;
+    fal   <- permute_graph prm g;
+    pi_gwco <$ djoinmap Com fal; 
 
-op HasHC (Ny : hc_prob) = exists w, IsHC (Ny, w).
+    return map fst pi_gwco;
+  }
+  
+  proc response(b : bool) : hc_resp = {
+    pi_w <- permute_witness prm w;
+    return if b then Left (prm, map snd pi_gwco) 
+                else Right (pi_w, map snd (prj_path pi_w pi_gwco));
+ } 
+}.
 
 
 
-
-lemma ishc_prop3 a  g w : IsHC a => a = (g,w) => prj_path w g = nseq K true.
-progress. elim H. smt.
-qed.
-
-
-axiom permute_graph_prop1 p n  : 
- permute_graph p (compl_graph n) = (compl_graph n).
+axiom permute_graph_prop1 p n : permute_graph p (compl_graph n) = (compl_graph n).
 
 axiom permute_graph_prop4  (g : graph) (p : permutation) :
  permute_graph (inv p) (permute_graph p g) = g.
 
 axiom permute_graph_prop2 p g : size (permute_graph p g) = size g.
 
-axiom permute_graph_prop3  g perm w : 
- IsHC (g, w) = IsHC (permute_graph perm g, permute_witness perm w).
+axiom permute_graph_prop3 g perm w : 
+ soundness_relation g w 
+   = soundness_relation (permute_graph perm g) (permute_witness perm w).
 
-axiom prj_lemma (g : graph) (w : hc_wit) (perm : permutation) : 
-   prj_path w g = prj_path (permute_witness perm w) (permute_graph perm g).
+axiom prj_lemma (g : graph) (w : hc_wit) (perm : permutation) :
+ completeness_relation g w 
+ => perm \in perm_d K 
+ => prj_path w g = prj_path (permute_witness perm w) (permute_graph perm g).
 
-axiom compl_graph_prop n : 0 <= n => IsHC ((compl_graph n), compl_graph_cyc n).
+axiom compl_graph_prop n : 0 <= n => completeness_relation (compl_graph n) (compl_graph_cyc n).
 
 axiom kjk prm w : prm \in perm_d K => uniq w => uniq (permute_witness prm w).
 
@@ -123,28 +128,3 @@ axiom lemma8 w (x : 'a list) (y : 'b list) : zip (prj_path w x) (prj_path w y) =
 
 
 
-
-module HonestProver : HonestProver  = {
-  var g : graph                 (* n*n adj. matrix *)
-  var prm : permutation         (* uniformly sampled permutation *)
-  var w : hc_wit                (* hamiltonian cycle *)
-  var fal : bool list           (* flattened and permuted g *)
-  var pi_gwco : (commitment * opening) list
-  var pi_w : hc_wit
-  
-  proc commitment(p_a : hc_prob, w_a : hc_wit)  = {
-    g <- p_a;
-    w     <- w_a;
-    prm   <$ perm_d K;
-    fal   <- permute_graph prm g;
-    pi_gwco <$ djoinmap Com fal; 
-
-    return map fst pi_gwco;
-  }
-  
-  proc response(b : bool) : hc_resp = {
-    pi_w <- permute_witness prm w;
-    return if b then Left (prm, map snd pi_gwco) 
-                else Right (pi_w, map snd (prj_path pi_w pi_gwco));
- } 
-}.
