aux/permutation.ec
@@ -1,9 +1,6 @@
 pragma Goals:printall.
-require import AllCore DBool Bool List Distr Int IntDiv Aux FSet.
+require import AllCore List Distr  .
 
-require import AllCore Distr FSet StdRing StdOrder StdBigop List.
-(*---*) import RField RealOrder Bigreal BRA.
-import BRM.
 
 type permutation = int -> int.
 
